WIP

concordium/src/concordium.rs
@@ -6,9 +6,9 @@
 #![feature(register_tool)]
 #![register_tool(hax)]
 
-#[hax_lib_macros::skip]
+#[hax_lib_macros::exclude]
 extern crate hax_lib_macros;
-#[hax_lib_macros::skip]
+#[hax_lib_macros::exclude]
 use hax_lib_macros::*;
 
 #[cfg(not(feature = "hacspec"))]
