ovn/src/ovn.rs
@@ -2,22 +2,51 @@
 #![feature(register_tool)]
 #![register_tool(hax)]
 
-#[hax_lib_macros::skip]
+#[hax_lib_macros::exclude]
 extern crate hax_lib_macros;
-#[hax_lib_macros::skip]
+#[hax_lib_macros::exclude]
 use hax_lib_macros::*;
 
-#[skip]
+#[exclude]
 use hacspec_concordium::*;
-#[skip]
+#[exclude]
 use hacspec_concordium_derive::*;
+
+pub enum vals {
+    MyVal,
+    YourVal (u32),
+    YourSecondVal (u32, u32),
+    StrangeVal {a : u32, b : u32, c : u32},
+}
+
+pub fn test_v() -> vals {
+    vals::YourVal(32)
+}
+
+pub fn test_vals ( x : vals) -> u32 {
+    match x {
+        vals::MyVal => 0,
+        vals::YourVal(x) => x,
+        vals::YourSecondVal(x, y) => y,
+        vals::StrangeVal { a, c, b } => c
+    }
+}
+
+pub struct alt_test {d : u32, e : u32, f : u32}
+
+pub fn test_alt_vals ( x : alt_test) -> u32 {
+    match x {
+        alt_test { d, f, e } => f
+    }
+}
 
 /** Interface for group implementation */
 pub trait Group {
-    type group_type: PartialEq + Eq + Clone + Copy + hacspec_concordium::Serialize;
+    type group_type: PartialEq + Eq + Clone + Copy + hacspec_concordium::Serialize
+        ;
 
-    const q: u32; // Prime order
-    const g: Self::group_type; // Generator (elemnent of group)
+    const q : u32; // Prime order
+    const g : Self::group_type; // Generator (elemnent of group)
 
     fn g_pow(x: u32) -> Self::group_type;
     fn pow(g: Self::group_type, x: u32) -> Self::group_type;
