concordium/proofs/ssprove/extraction/Hacspec_concordium_Concordium_traits.v
@@ -3,12 +3,12 @@ Set Warnings "-notation-overridden,-ambiguous-paths".
 From Crypt Require Import choice_type Package Prelude.
 Import PackageNotation.
 From extructures Require Import ord fset.
-From mathcomp Require Import ssrZ word.
+From mathcomp Require Import word_ssrZ word.
 From Jasmin Require Import word.
 
 From Coq Require Import ZArith.
 From Coq Require Import Strings.String.
-   Import List.ListNotations.
+Import List.ListNotations.
 Open Scope list_scope.
 Open Scope Z_scope.
 Open Scope bool_scope.
@@ -28,142 +28,177 @@ Require Import Crate.
 Export Crate.
 
 Class t_HasParameter (Self : choice_type) := {
-  size_loc : {fset Location} ;
-  size : forall {L1 I1}, both L1 I1 (Self) -> both (L1 :|: size_loc) I1 (int32) ;
+  f_size_loc : {fset Location} ;
+  f_size : forall {L1 I1}, both L1 I1 (v_Self) -> both (L1 :|: f_size_loc) I1 (int32) ;
 }.
+Hint Unfold f_size_loc.
 
 Class t_HasChainMetadata (Self : choice_type) := {
-  slot_time_loc : {fset Location} ;
-  slot_time : forall {L1 I1}, both L1 I1 (Self) -> both (L1 :|: slot_time_loc) I1 (t_Timestamp) ;
+  f_slot_time_loc : {fset Location} ;
+  f_slot_time : forall {L1 I1}, both L1 I1 (v_Self) -> both (L1 :|: f_slot_time_loc) I1 (t_Timestamp) ;
 }.
+Hint Unfold f_slot_time_loc.
 
 Class t_HasPolicy (Self : choice_type) := {
-  identity_provider_loc : {fset Location} ;
-  identity_provider : forall {L1 I1}, both L1 I1 (Self) -> both (L1 :|: identity_provider_loc) I1 (int32) ;
-  created_at_loc : {fset Location} ;
-  created_at : forall {L1 I1}, both L1 I1 (Self) -> both (L1 :|: created_at_loc) I1 (t_Timestamp) ;
-  valid_to_loc : {fset Location} ;
-  valid_to : forall {L1 I1}, both L1 I1 (Self) -> both (L1 :|: valid_to_loc) I1 (t_Timestamp) ;
-  next_item_loc : {fset Location} ;
-  next_item : forall {L1 L2 I1 I2}, both L1 I1 (Self) -> both L2 I2 (nseq int8 31) -> both (L1 :|: L2 :|: next_item_loc) (I1 :|: I2) ((t_Option ((t_AttributeTag × int8)) × nseq int8 31 × Self)) ;
+  f_identity_provider_loc : {fset Location} ;
+  f_identity_provider : forall {L1 I1}, both L1 I1 (v_Self) -> both (L1 :|: f_identity_provider_loc) I1 (int32) ;
+  f_created_at_loc : {fset Location} ;
+  f_created_at : forall {L1 I1}, both L1 I1 (v_Self) -> both (L1 :|: f_created_at_loc) I1 (t_Timestamp) ;
+  f_valid_to_loc : {fset Location} ;
+  f_valid_to : forall {L1 I1}, both L1 I1 (v_Self) -> both (L1 :|: f_valid_to_loc) I1 (t_Timestamp) ;
+  f_next_item_loc : {fset Location} ;
+  f_next_item : forall {L1 L2 I1 I2}, both L1 I1 (v_Self) -> both L2 I2 (nseq int8 31) -> both (L1 :|: L2 :|: f_next_item_loc) (I1 :|: I2) ((t_Option ((t_AttributeTag × int8)) × nseq int8 31 × v_Self)) ;
 }.
+Hint Unfold f_identity_provider_loc.
+Hint Unfold f_created_at_loc.
+Hint Unfold f_valid_to_loc.
+Hint Unfold f_next_item_loc.
 
 Class t_HasCommonData (Self : choice_type) := {
-  t_PolicyType : choice_type ;
-  t_PolicyType_t_HasPolicy :> t_HasPolicy (t_PolicyType) ;
-  t_PolicyType_t_Sized :> t_Sized (t_PolicyType) ;
-  t_MetadataType : choice_type ;
-  t_MetadataType_t_HasChainMetadata :> t_HasChainMetadata (t_MetadataType) ;
-  t_MetadataType_t_Sized :> t_Sized (t_MetadataType) ;
-  t_ParamType : choice_type ;
-  t_ParamType_t_Read :> t_Read (t_ParamType) ;
-  t_ParamType_t_HasParameter :> t_HasParameter (t_ParamType) ;
-  t_ParamType_t_Sized :> t_Sized (t_ParamType) ;
-  t_PolicyIteratorType : choice_type ;
-  t_PolicyIteratorType_t_ExactSizeIterator :> t_ExactSizeIterator (t_PolicyIteratorType) ;
-  t_PolicyIteratorType_t_Iterator :> t_Iterator (t_PolicyIteratorType) ;
-  t_PolicyIteratorType_t_Sized :> t_Sized (t_PolicyIteratorType) ;
-  policies_loc : {fset Location} ;
-  policies : forall {L1 I1}, both L1 I1 (Self) -> both (L1 :|: policies_loc) I1 (t_PolicyIteratorType) ;
-  metadata_loc : {fset Location} ;
-  metadata : forall {L1 I1}, both L1 I1 (Self) -> both (L1 :|: metadata_loc) I1 (t_MetadataType) ;
-  parameter_cursor_loc : {fset Location} ;
-  parameter_cursor : forall {L1 I1}, both L1 I1 (Self) -> both (L1 :|: parameter_cursor_loc) I1 (t_ParamType) ;
+  f_PolicyType : choice_type ;
+  f_PolicyType_t_HasPolicy :> t_HasPolicy (f_PolicyType) ;
+  f_PolicyType_t_Sized :> t_Sized (f_PolicyType) ;
+  f_MetadataType : choice_type ;
+  f_MetadataType_t_HasChainMetadata :> t_HasChainMetadata (f_MetadataType) ;
+  f_MetadataType_t_Sized :> t_Sized (f_MetadataType) ;
+  f_ParamType : choice_type ;
+  f_ParamType_t_Read :> t_Read (f_ParamType) ;
+  f_ParamType_t_HasParameter :> t_HasParameter (f_ParamType) ;
+  f_ParamType_t_Sized :> t_Sized (f_ParamType) ;
+  f_PolicyIteratorType : choice_type ;
+  f_PolicyIteratorType_t_ExactSizeIterator :> t_ExactSizeIterator (f_PolicyIteratorType) ;
+  f_PolicyIteratorType_t_Iterator :> t_Iterator (f_PolicyIteratorType) ;
+  f_PolicyIteratorType_t_Sized :> t_Sized (f_PolicyIteratorType) ;
+  f_policies_loc : {fset Location} ;
+  f_policies : forall {L1 I1}, both L1 I1 (v_Self) -> both (L1 :|: f_policies_loc) I1 (f_PolicyIteratorType) ;
+  f_metadata_loc : {fset Location} ;
+  f_metadata : forall {L1 I1}, both L1 I1 (v_Self) -> both (L1 :|: f_metadata_loc) I1 (f_MetadataType) ;
+  f_parameter_cursor_loc : {fset Location} ;
+  f_parameter_cursor : forall {L1 I1}, both L1 I1 (v_Self) -> both (L1 :|: f_parameter_cursor_loc) I1 (f_ParamType) ;
 }.
+Hint Unfold f_policies_loc.
+Hint Unfold f_metadata_loc.
+Hint Unfold f_parameter_cursor_loc.
 
 Class t_HasInitContext (Self : choice_type) := {
-  t_InitData : choice_type ;
-  t_InitData_t_Sized :> t_Sized (t_InitData) ;
-  open_loc : {fset Location} ;
-  open : forall {L1 I1}, both L1 I1 (t_InitData) -> both (L1 :|: open_loc) I1 (Self) ;
-  init_origin_loc : {fset Location} ;
-  init_origin : forall {L1 I1}, both L1 I1 (Self) -> both (L1 :|: init_origin_loc) I1 (t_AccountAddress) ;
+  f_InitData : choice_type ;
+  f_InitData_t_Sized :> t_Sized (f_InitData) ;
+  f_open_loc : {fset Location} ;
+  f_open : forall {L1 I1}, both L1 I1 (f_InitData) -> both (L1 :|: f_open_loc) I1 (v_Self) ;
+  f_init_origin_loc : {fset Location} ;
+  f_init_origin : forall {L1 I1}, both L1 I1 (v_Self) -> both (L1 :|: f_init_origin_loc) I1 (t_AccountAddress) ;
 }.
+Hint Unfold f_open_loc.
+Hint Unfold f_init_origin_loc.
 
 Class t_HasReceiveContext (Self : choice_type) := {
-  t_ReceiveData : choice_type ;
-  t_ReceiveData_t_Sized :> t_Sized (t_ReceiveData) ;
-  open_loc : {fset Location} ;
-  open : forall {L1 I1}, both L1 I1 (t_ReceiveData) -> both (L1 :|: open_loc) I1 (Self) ;
-  invoker_loc : {fset Location} ;
-  invoker : forall {L1 I1}, both L1 I1 (Self) -> both (L1 :|: invoker_loc) I1 (t_AccountAddress) ;
-  self_address_loc : {fset Location} ;
-  self_address : forall {L1 I1}, both L1 I1 (Self) -> both (L1 :|: self_address_loc) I1 (t_ContractAddress) ;
-  self_balance_loc : {fset Location} ;
-  self_balance : forall {L1 I1}, both L1 I1 (Self) -> both (L1 :|: self_balance_loc) I1 (t_Amount) ;
-  sender_loc : {fset Location} ;
-  sender : forall {L1 I1}, both L1 I1 (Self) -> both (L1 :|: sender_loc) I1 (t_Address) ;
-  owner_loc : {fset Location} ;
-  owner : forall {L1 I1}, both L1 I1 (Self) -> both (L1 :|: owner_loc) I1 (t_AccountAddress) ;
+  f_ReceiveData : choice_type ;
+  f_ReceiveData_t_Sized :> t_Sized (f_ReceiveData) ;
+  f_open_loc : {fset Location} ;
+  f_open : forall {L1 I1}, both L1 I1 (f_ReceiveData) -> both (L1 :|: f_open_loc) I1 (v_Self) ;
+  f_invoker_loc : {fset Location} ;
+  f_invoker : forall {L1 I1}, both L1 I1 (v_Self) -> both (L1 :|: f_invoker_loc) I1 (t_AccountAddress) ;
+  f_self_address_loc : {fset Location} ;
+  f_self_address : forall {L1 I1}, both L1 I1 (v_Self) -> both (L1 :|: f_self_address_loc) I1 (t_ContractAddress) ;
+  f_self_balance_loc : {fset Location} ;
+  f_self_balance : forall {L1 I1}, both L1 I1 (v_Self) -> both (L1 :|: f_self_balance_loc) I1 (t_Amount) ;
+  f_sender_loc : {fset Location} ;
+  f_sender : forall {L1 I1}, both L1 I1 (v_Self) -> both (L1 :|: f_sender_loc) I1 (t_Address) ;
+  f_owner_loc : {fset Location} ;
+  f_owner : forall {L1 I1}, both L1 I1 (v_Self) -> both (L1 :|: f_owner_loc) I1 (t_AccountAddress) ;
 }.
+Hint Unfold f_open_loc.
+Hint Unfold f_invoker_loc.
+Hint Unfold f_self_address_loc.
+Hint Unfold f_self_balance_loc.
+Hint Unfold f_sender_loc.
+Hint Unfold f_owner_loc.
 
 Class t_HasContractState (Self : choice_type) := {
-  t_ContractStateData : choice_type ;
-  t_ContractStateData_t_Sized :> t_Sized (t_ContractStateData) ;
-  open_loc : {fset Location} ;
-  open : forall {L1 I1}, both L1 I1 (t_ContractStateData) -> both (L1 :|: open_loc) I1 (Self) ;
-  size_loc : {fset Location} ;
-  size : forall {L1 I1}, both L1 I1 (Self) -> both (L1 :|: size_loc) I1 (int32) ;
-  truncate_loc : {fset Location} ;
-  truncate : forall {L1 L2 I1 I2}, both L1 I1 (Self) -> both L2 I2 (int32) -> both (L1 :|: L2 :|: truncate_loc) (I1 :|: I2) (Self) ;
-  reserve_loc : {fset Location} ;
-  reserve : forall {L1 L2 I1 I2}, both L1 I1 (Self) -> both L2 I2 (int32) -> both (L1 :|: L2 :|: reserve_loc) (I1 :|: I2) (('bool × Self)) ;
+  f_ContractStateData : choice_type ;
+  f_ContractStateData_t_Sized :> t_Sized (f_ContractStateData) ;
+  f_open_loc : {fset Location} ;
+  f_open : forall {L1 I1}, both L1 I1 (f_ContractStateData) -> both (L1 :|: f_open_loc) I1 (v_Self) ;
+  f_size_loc : {fset Location} ;
+  f_size : forall {L1 I1}, both L1 I1 (v_Self) -> both (L1 :|: f_size_loc) I1 (int32) ;
+  f_truncate_loc : {fset Location} ;
+  f_truncate : forall {L1 L2 I1 I2}, both L1 I1 (v_Self) -> both L2 I2 (int32) -> both (L1 :|: L2 :|: f_truncate_loc) (I1 :|: I2) (v_Self) ;
+  f_reserve_loc : {fset Location} ;
+  f_reserve : forall {L1 L2 I1 I2}, both L1 I1 (v_Self) -> both L2 I2 (int32) -> both (L1 :|: L2 :|: f_reserve_loc) (I1 :|: I2) (('bool × v_Self)) ;
 }.
+Hint Unfold f_open_loc.
+Hint Unfold f_size_loc.
+Hint Unfold f_truncate_loc.
+Hint Unfold f_reserve_loc.
 
 Class t_HasLogger (Self : choice_type) := {
-  init_loc : {fset Location} ;
-  init : forall {L1 I1}, both (L1 :|: init_loc) I1 (Self) ;
-  log_raw_loc : {fset Location} ;
-  log_raw : forall {L1 L2 I1 I2}, both L1 I1 (Self) -> both L2 I2 (seq int8) -> both (L1 :|: L2 :|: log_raw_loc) (I1 :|: I2) ((t_Result ('unit) (t_LogError) × Self)) ;
-  log_loc : {fset Location} ;
-  log : forall {L1 L2 I1 I2}, both L1 I1 (Self) -> both L2 I2 (S) -> both (L1 :|: L2 :|: log_loc) (I1 :|: I2) ((t_Result ('unit) (t_LogError) × Self)) ;
+  f_init_loc : {fset Location} ;
+  f_init : forall {L1 I1}, both (L1 :|: f_init_loc) I1 (v_Self) ;
+  f_log_raw_loc : {fset Location} ;
+  f_log_raw : forall {L1 L2 I1 I2}, both L1 I1 (v_Self) -> both L2 I2 (seq int8) -> both (L1 :|: L2 :|: f_log_raw_loc) (I1 :|: I2) ((t_Result ('unit) (t_LogError) × v_Self)) ;
+  f_log_loc : {fset Location} ;
+  f_log : forall {L1 L2 I1 I2}, both L1 I1 (v_Self) -> both L2 I2 (v_S) -> both (L1 :|: L2 :|: f_log_loc) (I1 :|: I2) ((t_Result ('unit) (t_LogError) × v_Self)) ;
 }.
+Hint Unfold f_init_loc.
+Hint Unfold f_log_raw_loc.
+Hint Unfold f_log_loc.
 
 Class t_HasActions (Self : choice_type) := {
-  accept_loc : {fset Location} ;
-  accept : forall {L1 I1}, both (L1 :|: accept_loc) I1 (Self) ;
-  simple_transfer_loc : {fset Location} ;
-  simple_transfer : forall {L1 L2 I1 I2}, both L1 I1 (t_AccountAddress) -> both L2 I2 (t_Amount) -> both (L1 :|: L2 :|: simple_transfer_loc) (I1 :|: I2) (Self) ;
-  send_raw_loc : {fset Location} ;
-  send_raw : forall {L1 L2 L3 L4 I1 I2 I3 I4}, both L1 I1 (t_ContractAddress) -> both L2 I2 (t_ReceiveName) -> both L3 I3 (t_Amount) -> both L4 I4 (seq int8) -> both (L1 :|: L2 :|: L3 :|: L4 :|: send_raw_loc) (I1 :|: I2 :|: I3 :|: I4) (Self) ;
-  and_then_loc : {fset Location} ;
-  and_then : forall {L1 L2 I1 I2}, both L1 I1 (Self) -> both L2 I2 (Self) -> both (L1 :|: L2 :|: and_then_loc) (I1 :|: I2) (Self) ;
-  or_else_loc : {fset Location} ;
-  or_else : forall {L1 L2 I1 I2}, both L1 I1 (Self) -> both L2 I2 (Self) -> both (L1 :|: L2 :|: or_else_loc) (I1 :|: I2) (Self) ;
+  f_accept_loc : {fset Location} ;
+  f_accept : forall {L1 I1}, both (L1 :|: f_accept_loc) I1 (v_Self) ;
+  f_simple_transfer_loc : {fset Location} ;
+  f_simple_transfer : forall {L1 L2 I1 I2}, both L1 I1 (t_AccountAddress) -> both L2 I2 (t_Amount) -> both (L1 :|: L2 :|: f_simple_transfer_loc) (I1 :|: I2) (v_Self) ;
+  f_send_raw_loc : {fset Location} ;
+  f_send_raw : forall {L1 L2 L3 L4 I1 I2 I3 I4}, both L1 I1 (t_ContractAddress) -> both L2 I2 (t_ReceiveName) -> both L3 I3 (t_Amount) -> both L4 I4 (seq int8) -> both (L1 :|: L2 :|: L3 :|: L4 :|: f_send_raw_loc) (I1 :|: I2 :|: I3 :|: I4) (v_Self) ;
+  f_and_then_loc : {fset Location} ;
+  f_and_then : forall {L1 L2 I1 I2}, both L1 I1 (v_Self) -> both L2 I2 (v_Self) -> both (L1 :|: L2 :|: f_and_then_loc) (I1 :|: I2) (v_Self) ;
+  f_or_else_loc : {fset Location} ;
+  f_or_else : forall {L1 L2 I1 I2}, both L1 I1 (v_Self) -> both L2 I2 (v_Self) -> both (L1 :|: L2 :|: f_or_else_loc) (I1 :|: I2) (v_Self) ;
 }.
+Hint Unfold f_accept_loc.
+Hint Unfold f_simple_transfer_loc.
+Hint Unfold f_send_raw_loc.
+Hint Unfold f_and_then_loc.
+Hint Unfold f_or_else_loc.
 
 Class t_UnwrapAbort (Self : choice_type) := {
-  t_Unwrap : choice_type ;
-  t_Unwrap_t_Sized :> t_Sized (t_Unwrap) ;
-  unwrap_abort_loc : {fset Location} ;
-  unwrap_abort : forall {L1 I1}, both L1 I1 (Self) -> both (L1 :|: unwrap_abort_loc) I1 (t_Unwrap) ;
+  f_Unwrap : choice_type ;
+  f_Unwrap_t_Sized :> t_Sized (f_Unwrap) ;
+  f_unwrap_abort_loc : {fset Location} ;
+  f_unwrap_abort : forall {L1 I1}, both L1 I1 (v_Self) -> both (L1 :|: f_unwrap_abort_loc) I1 (f_Unwrap) ;
 }.
+Hint Unfold f_unwrap_abort_loc.
 
 Class t_ExpectReport (Self : choice_type) := {
-  t_Unwrap : choice_type ;
-  t_Unwrap_t_Sized :> t_Sized (t_Unwrap) ;
-  expect_report_loc : {fset Location} ;
-  expect_report : forall {L1 L2 I1 I2}, both L1 I1 (Self) -> both L2 I2 (chString) -> both (L1 :|: L2 :|: expect_report_loc) (I1 :|: I2) (t_Unwrap) ;
+  f_Unwrap : choice_type ;
+  f_Unwrap_t_Sized :> t_Sized (f_Unwrap) ;
+  f_expect_report_loc : {fset Location} ;
+  f_expect_report : forall {L1 L2 I1 I2}, both L1 I1 (v_Self) -> both L2 I2 (chString) -> both (L1 :|: L2 :|: f_expect_report_loc) (I1 :|: I2) (f_Unwrap) ;
 }.
+Hint Unfold f_expect_report_loc.
 
 Class t_ExpectErrReport (Self : choice_type) := {
-  t_Unwrap : choice_type ;
-  t_Unwrap_t_Sized :> t_Sized (t_Unwrap) ;
-  expect_err_report_loc : {fset Location} ;
-  expect_err_report : forall {L1 L2 I1 I2}, both L1 I1 (Self) -> both L2 I2 (chString) -> both (L1 :|: L2 :|: expect_err_report_loc) (I1 :|: I2) (t_Unwrap) ;
+  f_Unwrap : choice_type ;
+  f_Unwrap_t_Sized :> t_Sized (f_Unwrap) ;
+  f_expect_err_report_loc : {fset Location} ;
+  f_expect_err_report : forall {L1 L2 I1 I2}, both L1 I1 (v_Self) -> both L2 I2 (chString) -> both (L1 :|: L2 :|: f_expect_err_report_loc) (I1 :|: I2) (f_Unwrap) ;
 }.
+Hint Unfold f_expect_err_report_loc.
 
 Class t_ExpectNoneReport (Self : choice_type) := {
-  expect_none_report_loc : {fset Location} ;
-  expect_none_report : forall {L1 L2 I1 I2}, both L1 I1 (Self) -> both L2 I2 (chString) -> both (L1 :|: L2 :|: expect_none_report_loc) (I1 :|: I2) ('unit) ;
+  f_expect_none_report_loc : {fset Location} ;
+  f_expect_none_report : forall {L1 L2 I1 I2}, both L1 I1 (v_Self) -> both L2 I2 (chString) -> both (L1 :|: L2 :|: f_expect_none_report_loc) (I1 :|: I2) ('unit) ;
 }.
+Hint Unfold f_expect_none_report_loc.
 
 Class t_SerialCtx (Self : choice_type) := {
-  serial_ctx_loc : {fset Location} ;
-  serial_ctx : forall {L1 L2 L3 I1 I2 I3}, both L1 I1 (Self) -> both L2 I2 (t_SizeLength) -> both L3 I3 (W) -> both (L1 :|: L2 :|: L3 :|: serial_ctx_loc) (I1 :|: I2 :|: I3) ((t_Result ('unit) (t_Err) × W)) ;
+  f_serial_ctx_loc : {fset Location} ;
+  f_serial_ctx : forall {L1 L2 L3 I1 I2 I3}, both L1 I1 (v_Self) -> both L2 I2 (t_SizeLength) -> both L3 I3 (v_W) -> both (L1 :|: L2 :|: L3 :|: f_serial_ctx_loc) (I1 :|: I2 :|: I3) ((t_Result ('unit) (f_Err) × v_W)) ;
 }.
+Hint Unfold f_serial_ctx_loc.
 
 Class t_DeserialCtx (Self : choice_type) := {
-  deserial_ctx_loc : {fset Location} ;
-  deserial_ctx : forall {L1 L2 L3 I1 I2 I3}, both L1 I1 (t_SizeLength) -> both L2 I2 ('bool) -> both L3 I3 (R) -> both (L1 :|: L2 :|: L3 :|: deserial_ctx_loc) (I1 :|: I2 :|: I3) ((t_Result (Self) (t_ParseError) × R)) ;
+  f_deserial_ctx_loc : {fset Location} ;
+  f_deserial_ctx : forall {L1 L2 L3 I1 I2 I3}, both L1 I1 (t_SizeLength) -> both L2 I2 ('bool) -> both L3 I3 (v_R) -> both (L1 :|: L2 :|: L3 :|: f_deserial_ctx_loc) (I1 :|: I2 :|: I3) ((t_Result (v_Self) (t_ParseError) × v_R)) ;
 }.
+Hint Unfold f_deserial_ctx_loc.
