concordium/proofs/fstar/extraction/Hacspec_concordium.Concordium_types.Sealed.fst
@@ -1,0 +1,13 @@
+module Hacspec_concordium.Concordium_types.Sealed
+#set-options "--fuel 0 --ifuel 1 --z3rlimit 15"
+open Core
+
+class t_ContextType (#v_Self: Type) = {
+  [@@@ FStar.Tactics.Typeclasses.no_method]_super_734339128:t_ContextType v_Self
+}
+
+let impl: t_ContextType Hacspec_concordium.Concordium_types.t_InitContextExtern =
+  { __marker_trait = () }
+
+let impl_1: t_ContextType Hacspec_concordium.Concordium_types.t_ReceiveContextExtern =
+  { __marker_trait = () }
