concordium/proofs/fstar/extraction/Hacspec_concordium.Concordium_types.fst
@@ -1,0 +1,53 @@
+module Hacspec_concordium.Concordium_types
+#set-options "--fuel 0 --ifuel 1 --z3rlimit 15"
+open Core
+
+type t_ContractState = { f_current_contract_state_position:u32 }
+
+type t_Parameter = { f_current_parameter_position:u32 }
+
+type t_AttributesCursor = {
+  f_current_attribute_cursor_position:u32;
+  f_remaining_items:u16
+}
+
+type t_Logger = { f__private_logger:Prims.unit }
+
+type t_LogError =
+  | LogError_Full : t_LogError
+  | LogError_Malformed : t_LogError
+
+type t_NotPayableError = | NotPayableError : t_NotPayableError
+
+type t_Action = { f__private_action:u32 }
+
+let impl__tag (self: t_Action) : u32 = self.f__private_action
+
+let v____: Prims.unit = ()
+
+let v______refinement (error_code: Core.Num.Nonzero.t_NonZeroI32) : bool = true
+
+type t_Reject = { f_error_code:f_error_code: Core.Num.Nonzero.t_NonZeroI32{true} }
+
+let impl_1: Core.Default.t_Default t_Reject = { __marker_trait = () }
+
+let t_ReceiveResult
+      (#v_A: Type)
+      (#[FStar.Tactics.Typeclasses.tcresolve ()] ii0: Core.Marker.t_Sized v_A)
+     = Core.Result.t_Result v_A t_Reject
+
+let t_InitResult
+      (#v_S: Type)
+      (#[FStar.Tactics.Typeclasses.tcresolve ()] ii0: Core.Marker.t_Sized v_S)
+     = Core.Result.t_Result v_S t_Reject
+
+type t_ExternContext
+  (#v_T: Type) {| _: Core.Marker.t_Sized v_T |}
+  {| _: Hacspec_concordium.Concordium_types.Sealed.t_ContextType v_T |}
+  = { f_marker:Core.Marker.t_PhantomData v_T }
+
+type t_ChainMetaExtern = | ChainMetaExtern : t_ChainMetaExtern
+
+type t_InitContextExtern = | InitContextExtern : t_InitContextExtern
+
+type t_ReceiveContextExtern = | ReceiveContextExtern : t_ReceiveContextExtern
