concordium/proofs/fstar/extraction/Hacspec_concordium.Constants.fst
@@ -1,0 +1,9 @@
+module Hacspec_concordium.Constants
+#set-options "--fuel 0 --ifuel 1 --z3rlimit 15"
+open Core
+
+let v_MAX_CONTRACT_STATE_SIZE: u32 = 16384ul
+
+let v_MAX_LOG_SIZE: usize = sz 512
+
+let v_MAX_NUM_LOGS: usize = sz 64
