concordium/proofs/fstar/extraction/Hacspec_concordium.fst
@@ -1,0 +1,5 @@
+module Hacspec_concordium
+#set-options "--fuel 0 --ifuel 1 --z3rlimit 15"
+open Core
+
+let trap: Rust_primitives.Hax.t_Never = Core.Intrinsics.abort
